Further adjustments for new term definition

ProofLibrary/ChaseSequence/Termination/MfaLike.lean
@@ -18,7 +18,45 @@ namespace ConstantMapping
 
   variable {sig : Signature} [DecidableEq sig.C] [DecidableEq sig.V]
 
-  def apply_ground_term (g : ConstantMapping sig) (t : GroundTerm sig) : GroundTerm sig := t.mapLeaves g
+  def apply_pre_ground_term (g : ConstantMapping sig) (t : PreGroundTerm sig) : PreGroundTerm sig := t.mapLeaves (fun c => (g c).val)
+
+  mutual
+
+    theorem apply_pre_ground_term_arity_ok (g : ConstantMapping sig) (t : FiniteTree (SkolemFS sig) sig.C) (arity_ok : PreGroundTerm.arity_ok t) : PreGroundTerm.arity_ok (g.apply_pre_ground_term t) := by
+      cases t with
+      | leaf c =>
+        unfold apply_pre_ground_term
+        unfold FiniteTree.mapLeaves
+        exact (g c).property
+      | inner f ts =>
+        unfold PreGroundTerm.arity_ok at arity_ok
+        rw [Bool.and_eq_true] at arity_ok
+        unfold apply_pre_ground_term
+        unfold FiniteTree.mapLeaves
+        unfold PreGroundTerm.arity_ok
+        rw [Bool.and_eq_true]
+        constructor
+        . rw [FiniteTree.length_mapLeavesList]
+          exact arity_ok.left
+        . apply apply_pre_ground_term_list_arity_ok
+          exact arity_ok.right
+
+    theorem apply_pre_ground_term_list_arity_ok (g : ConstantMapping sig) (ts : FiniteTreeList (SkolemFS sig) sig.C) (arity_ok : PreGroundTerm.arity_ok_list ts) : PreGroundTerm.arity_ok_list (FiniteTree.mapLeavesList (fun c => (g c).val) ts) := by
+      cases ts with
+      | nil => simp [FiniteTree.mapLeavesList, PreGroundTerm.arity_ok_list]
+      | cons hd tl =>
+        unfold PreGroundTerm.arity_ok_list at arity_ok
+        rw [Bool.and_eq_true] at arity_ok
+        unfold FiniteTree.mapLeavesList
+        unfold PreGroundTerm.arity_ok_list
+        rw [Bool.and_eq_true]
+        constructor
+        . apply apply_pre_ground_term_arity_ok; exact arity_ok.left
+        . apply apply_pre_ground_term_list_arity_ok; exact arity_ok.right
+
+  end
+
+  def apply_ground_term (g : ConstantMapping sig) (t : GroundTerm sig) : GroundTerm sig := ⟨g.apply_pre_ground_term t.val, g.apply_pre_ground_term_arity_ok t.val t.property⟩
 
   theorem apply_ground_term_swap_apply_skolem_term (g : ConstantMapping sig) (subs : GroundSubstitution sig) : ∀ t, (∀ c, t ≠ SkolemTerm.const c) -> g.apply_ground_term (subs.apply_skolem_term t) = GroundSubstitution.apply_skolem_term (g.apply_ground_term ∘ subs) t := by
     intro t
@@ -32,6 +70,7 @@ namespace ConstantMapping
       intros
       conv => left; unfold ConstantMapping.apply_ground_term; unfold FiniteTree.mapLeaves; unfold GroundSubstitution.apply_skolem_term
       conv => right; unfold GroundSubstitution.apply_skolem_term
+      simp only [apply_pre_ground_term, FiniteTree.mapLeaves]
       simp
       rw [FiniteTree.mapLeavesList_fromList_eq_fromList_map]
       unfold ConstantMapping.apply_ground_term
@@ -66,12 +105,16 @@ namespace ConstantMapping
       unfold VarOrConst.skolemize
       unfold GroundSubstitution.apply_skolem_term
       unfold ConstantMapping.apply_ground_term
+      unfold ConstantMapping.apply_pre_ground_term
       unfold FiniteTree.mapLeaves
+      unfold GroundTerm.const
+      apply Subtype.eq
       simp only
       rcases h with ⟨c, g_eq, mem_a_eq⟩
       rw [g_eq]
-      apply mem_a_eq
-      exact voc_mem
+      rw [mem_a_eq d]
+      . simp [GroundTerm.const]
+      . exact voc_mem
 
   def apply_fact_set (g : ConstantMapping sig) (fs : FactSet sig) : FactSet sig := fun f => ∃ f', f' ∈ fs ∧ f = g.apply_fact f'
 
@@ -181,73 +224,33 @@ section ArgumentsForImages
 
     variable [DecidableEq sig.V]
 
-    def arguments_for_term (g : StrictConstantMapping sig) (possible_constants : List sig.C) (t : GroundTerm sig) : List (GroundTerm sig) :=
-      t.cases (
-        fun c => (g.arguments_for_constant possible_constants c).map (fun arg => GroundTerm.const arg)
-      ) (
-        fun f ts arity_ok =>
-          let args : List (List (GroundTerm sig)) := ts.foldl (fun acc (t' : GroundTerm sig) =>
-            have : t'.val.depth < t.val.depth := by
-              sorry
-            /-   conv => right; unfold FiniteTree.depth -/
-            /-   simp only [eq_val] -/
-            /-   rw [Nat.add_comm] -/
-            /-   apply Nat.lt_add_one_of_le -/
-            /-   apply FiniteTree.depth_le_depthList_of_mem -/
-            /-   unfold ts at mem -/
-            /-   rw [List.mem_map] at mem -/
-            /-   rcases mem with ⟨s, s_mem, t_eq⟩ -/
-            /-   simp at t_eq -/
-            /-   rw [← t_eq] -/
-            /-   unfold List.attach at s_mem -/
-            /-   unfold List.attachWith at s_mem -/
-            /-   rw [List.mem_pmap] at s_mem -/
-            /-   rcases s_mem with ⟨_, s_mem, s_eq⟩ -/
-            /-   rw [← s_eq] -/
-            /-   exact s_mem -/
-            /-   sorry -/
-            (g.arguments_for_term possible_constants t').flatMap (fun arg =>
-              acc.map (fun args =>
-                arg :: args
-              )
-            )
-          ) [[]]
-          args.map (fun ts =>
-            GroundTerm.func f ts (by sorry)
+    mutual
+      def arguments_for_pre_term (g : StrictConstantMapping sig) (possible_constants : List sig.C) : FiniteTree (SkolemFS sig) sig.C -> List (PreGroundTerm sig)
+      | .leaf c => (g.arguments_for_constant possible_constants c).map (fun arg => .leaf arg)
+      | .inner func ts =>
+        (g.arguments_for_pre_term_list possible_constants ts).map (fun ts =>
+          .inner func (FiniteTreeList.fromList ts)
+        )
+      def arguments_for_pre_term_list (g : StrictConstantMapping sig) (possible_constants : List sig.C) : FiniteTreeList (SkolemFS sig) sig.C -> List (List (PreGroundTerm sig))
+      | .nil => [[]]
+      | .cons hd tl =>
+        let arguments_tail := g.arguments_for_pre_term_list possible_constants tl
+        (g.arguments_for_pre_term possible_constants hd).flatMap (fun arg =>
+          arguments_tail.map (fun arg_list =>
+            arg :: arg_list
           )
-          /- ts.flatMap (fun t => sorry) -/
-      )
-      termination_by t.val.depth
-    /- | .const c => sorry -/
-    /- | .func f ts arity => sorry -/
-
-    /- mutual -/
-    /-   def arguments_for_term (g : StrictConstantMapping sig) (possible_constants : List sig.C) : FiniteTree (SkolemFS sig) sig.C -> List (GroundTerm sig) -/
-    /-   | .leaf c => (g.arguments_for_constant possible_constants c).map (fun arg => .leaf arg) -/
-    /-   | .inner func ts => -/
-    /-     (g.arguments_for_term_list possible_constants ts).map (fun ts => -/
-    /-       .inner func (FiniteTreeList.fromList ts) -/
-    /-     ) -/
-    /-   def arguments_for_term_list (g : StrictConstantMapping sig) (possible_constants : List sig.C) : FiniteTreeList (SkolemFS sig) sig.C -> List (List (GroundTerm sig)) -/
-    /-   | .nil => [[]] -/
-    /-   | .cons hd tl => -/
-    /-     let arguments_tail := g.arguments_for_term_list possible_constants tl -/
-    /-     (g.arguments_for_term possible_constants hd).flatMap (fun arg => -/
-    /-       arguments_tail.map (fun arg_list => -/
-    /-         arg :: arg_list -/
-    /-       ) -/
-    /-     ) -/
-    /- end -/
+        )
+    end
 
     mutual
-      theorem apply_to_arguments_yields_original_term (g : StrictConstantMapping sig) (possible_constants : List sig.C) (term : FiniteTree (SkolemFS sig) sig.C) :
-          ∀ arg, arg ∈ g.arguments_for_term possible_constants term ↔ ((∀ c, c ∈ arg.leaves -> c ∈ possible_constants) ∧ g.toConstantMapping.apply_ground_term arg = term) := by
+      theorem apply_to_arguments_yields_original_pre_term (g : StrictConstantMapping sig) (possible_constants : List sig.C) (term : FiniteTree (SkolemFS sig) sig.C) :
+          ∀ arg, arg ∈ g.arguments_for_pre_term possible_constants term ↔ ((∀ c, c ∈ arg.leaves -> c ∈ possible_constants) ∧ g.toConstantMapping.apply_pre_ground_term arg = term) := by
         intro arg
         constructor
         . intro h
           cases term with
           | leaf c =>
-            unfold arguments_for_term at h
+            unfold arguments_for_pre_term at h
             rw [List.mem_map] at h
             rcases h with ⟨a, a_mem, arg_eq⟩
             rw [apply_to_arguments_yields_original_constant] at a_mem
@@ -259,16 +262,16 @@ section ArgumentsForImages
               rw [d_mem]
               exact a_mem.left
             . rw [← arg_eq]
-              unfold ConstantMapping.apply_ground_term
+              unfold ConstantMapping.apply_pre_ground_term
               unfold FiniteTree.mapLeaves
               unfold toConstantMapping
               rw [a_mem.right]
               rfl
           | inner func ts =>
-            unfold arguments_for_term at h
+            unfold arguments_for_pre_term at h
             rw [List.mem_map] at h
             rcases h with ⟨a, a_mem, arg_eq⟩
-            rw [apply_to_arguments_yields_original_term_list] at a_mem
+            rw [apply_to_arguments_yields_original_pre_term_list] at a_mem
             constructor
             . intro d d_mem
               rw [← arg_eq] at d_mem
@@ -276,13 +279,13 @@ section ArgumentsForImages
               apply a_mem.left
               exact d_mem
             . rw [← arg_eq]
-              unfold ConstantMapping.apply_ground_term
+              unfold ConstantMapping.apply_pre_ground_term
               unfold FiniteTree.mapLeaves
               rw [a_mem.right]
         . intro h
           cases term with
           | leaf c =>
-            unfold arguments_for_term
+            unfold arguments_for_pre_term
             rw [List.mem_map]
             cases arg with
             | leaf d =>
@@ -294,24 +297,24 @@ section ArgumentsForImages
                   unfold FiniteTree.leaves
                   simp
                 . have r := h.right
-                  unfold ConstantMapping.apply_ground_term at r
+                  unfold ConstantMapping.apply_pre_ground_term at r
                   unfold toConstantMapping at r
                   unfold FiniteTree.mapLeaves at r
                   injection r with r
               . rfl
             | inner func args =>
               have contra := h.right
-              simp [ConstantMapping.apply_ground_term, FiniteTree.mapLeaves] at contra
+              simp [ConstantMapping.apply_pre_ground_term, FiniteTree.mapLeaves] at contra
           | inner func ts =>
-            unfold arguments_for_term
+            unfold arguments_for_pre_term
             rw [List.mem_map]
             cases arg with
             | leaf d =>
               have contra := h.right
-              simp [ConstantMapping.apply_ground_term, FiniteTree.mapLeaves, toConstantMapping, GroundTerm.const] at contra
+              simp [ConstantMapping.apply_pre_ground_term, FiniteTree.mapLeaves, toConstantMapping, GroundTerm.const] at contra
             | inner func' args =>
               exists args
-              rw [apply_to_arguments_yields_original_term_list]
+              rw [apply_to_arguments_yields_original_pre_term_list]
               constructor
               . constructor
                 . intro d d_mem
@@ -320,36 +323,36 @@ section ArgumentsForImages
                   rw [FiniteTreeList.toListFromListIsId] at d_mem
                   exact d_mem
                 . have r := h.right
-                  unfold ConstantMapping.apply_ground_term at r
+                  unfold ConstantMapping.apply_pre_ground_term at r
                   unfold FiniteTree.mapLeaves at r
                   injection r with func_eq args_eq
                   rw [FiniteTreeList.toListFromListIsId]
                   exact args_eq
               . have r := h.right
-                unfold ConstantMapping.apply_ground_term at r
+                unfold ConstantMapping.apply_pre_ground_term at r
                 unfold FiniteTree.mapLeaves at r
                 injection r with func_eq args_eq
                 rw [FiniteTreeList.toListFromListIsId]
                 rw [func_eq]
 
-      theorem apply_to_arguments_yields_original_term_list (g : StrictConstantMapping sig) (possible_constants : List sig.C) (ts : FiniteTreeList (SkolemFS sig) sig.C) :
-          ∀ args, args ∈ g.arguments_for_term_list possible_constants ts ↔ ((∀ c, c ∈ (FiniteTree.leavesList (FiniteTreeList.fromList args)) -> c ∈ possible_constants) ∧ ((FiniteTree.mapLeavesList (fun leaf => g.toConstantMapping leaf) (FiniteTreeList.fromList args)) = ts)) := by
+      theorem apply_to_arguments_yields_original_pre_term_list (g : StrictConstantMapping sig) (possible_constants : List sig.C) (ts : FiniteTreeList (SkolemFS sig) sig.C) :
+          ∀ args, args ∈ g.arguments_for_pre_term_list possible_constants ts ↔ ((∀ c, c ∈ (FiniteTree.leavesList (FiniteTreeList.fromList args)) -> c ∈ possible_constants) ∧ ((FiniteTree.mapLeavesList (fun leaf => g.toConstantMapping leaf) (FiniteTreeList.fromList args)) = ts)) := by
         intro args
         constructor
         . intro h
           cases ts with
           | nil =>
-            simp [arguments_for_term_list] at h
+            simp [arguments_for_pre_term_list] at h
             rw [h]
             simp [FiniteTreeList.fromList, FiniteTree.mapLeavesList, FiniteTree.leavesList]
           | cons hd tl =>
-            unfold arguments_for_term_list at h
+            unfold arguments_for_pre_term_list at h
             rw [List.mem_flatMap] at h
             rcases h with ⟨hd_arg, hd_arg_mem, args_mem⟩
             rw [List.mem_map] at args_mem
             rcases args_mem with ⟨tl_args, tl_args_mem, args_eq⟩
-            rw [apply_to_arguments_yields_original_term] at hd_arg_mem
-            rw [apply_to_arguments_yields_original_term_list] at tl_args_mem
+            rw [apply_to_arguments_yields_original_pre_term] at hd_arg_mem
+            rw [apply_to_arguments_yields_original_pre_term_list] at tl_args_mem
             rw [← args_eq]
             constructor
             . intro d d_mem
@@ -361,14 +364,14 @@ section ArgumentsForImages
               | inr d_mem => apply tl_args_mem.left; exact d_mem
             . unfold FiniteTreeList.fromList
               unfold FiniteTree.mapLeavesList
-              unfold ConstantMapping.apply_ground_term at hd_arg_mem
+              unfold ConstantMapping.apply_pre_ground_term at hd_arg_mem
               rw [hd_arg_mem.right]
               rw [tl_args_mem.right]
         . intro h
           cases ts with
           | nil =>
             cases args with
-            | nil => simp [arguments_for_term_list]
+            | nil => simp [arguments_for_pre_term_list]
             | cons hd_arg tl_arg =>
               have r := h.right
               simp [FiniteTreeList.fromList, FiniteTree.mapLeavesList] at r
@@ -378,14 +381,14 @@ section ArgumentsForImages
               have r := h.right
               simp [FiniteTreeList.fromList, FiniteTree.mapLeavesList] at r
             | cons hd_arg tl_arg =>
-              unfold arguments_for_term_list
+              unfold arguments_for_pre_term_list
               unfold FiniteTreeList.fromList at h
               unfold FiniteTree.leavesList at h
               unfold FiniteTree.mapLeavesList at h
               rw [List.mem_flatMap]
               exists hd_arg
               constructor
-              . rw [apply_to_arguments_yields_original_term]
+              . rw [apply_to_arguments_yields_original_pre_term]
                 constructor
                 . intro d d_mem
                   apply h.left
@@ -396,7 +399,7 @@ section ArgumentsForImages
               . rw [List.mem_map]
                 exists tl_arg
                 simp only [and_true]
-                rw [apply_to_arguments_yields_original_term_list]
+                rw [apply_to_arguments_yields_original_pre_term_list]
                 constructor
                 . intro d d_mem
                   apply h.left
@@ -406,13 +409,13 @@ section ArgumentsForImages
                 . injection h.right
     end
 
-    theorem arguments_for_term_list_length_preserved (g : StrictConstantMapping sig) (possible_constants : List sig.C) (ts : FiniteTreeList (SkolemFS sig) sig.C) :
-        ∀ res, res ∈ (g.arguments_for_term_list possible_constants ts) -> res.length = ts.toList.length := by
+    theorem arguments_for_pre_term_list_length_preserved (g : StrictConstantMapping sig) (possible_constants : List sig.C) (ts : FiniteTreeList (SkolemFS sig) sig.C) :
+        ∀ res, res ∈ (g.arguments_for_pre_term_list possible_constants ts) -> res.length = ts.toList.length := by
       cases ts with
-      | nil => simp [arguments_for_term_list, FiniteTreeList.toList]
+      | nil => simp [arguments_for_pre_term_list, FiniteTreeList.toList]
       | cons hd tl =>
         intro res res_mem
-        unfold arguments_for_term_list at res_mem
+        unfold arguments_for_pre_term_list at res_mem
         rw [List.mem_flatMap] at res_mem
         rcases res_mem with ⟨arg, arg_for_hd, res_mem⟩
         rw [List.mem_map] at res_mem
@@ -422,20 +425,160 @@ section ArgumentsForImages
         rw [List.length_cons]
         rw [List.length_cons]
         rw [Nat.add_right_cancel_iff]
-        exact g.arguments_for_term_list_length_preserved possible_constants tl args args_for_tl
+        exact g.arguments_for_pre_term_list_length_preserved possible_constants tl args args_for_tl
 
+    mutual
+
+      theorem arguments_for_pre_term_arity_ok (g : StrictConstantMapping sig) (possible_constants : List sig.C) (t : FiniteTree (SkolemFS sig) sig.C) (arity_ok : PreGroundTerm.arity_ok t) : ∀ t', t' ∈ (g.arguments_for_pre_term possible_constants t) -> PreGroundTerm.arity_ok t' := by
+        intro t' t'_mem
+        unfold arguments_for_pre_term at t'_mem
+        cases t with
+        | leaf c =>
+          rw [List.mem_map] at t'_mem
+          rcases t'_mem with ⟨d, d_mem, t'_eq⟩
+          rw [← t'_eq]
+          simp [PreGroundTerm.arity_ok]
+        | inner f ts =>
+          unfold PreGroundTerm.arity_ok at arity_ok
+          rw [Bool.and_eq_true] at arity_ok
+          rw [List.mem_map] at t'_mem
+          rcases t'_mem with ⟨ts', ts'_mem, t'_eq⟩
+          rw [← t'_eq]
+          simp only [PreGroundTerm.arity_ok]
+          rw [Bool.and_eq_true]
+          constructor
+          . rw [FiniteTreeList.fromListToListIsId]
+            rw [g.arguments_for_pre_term_list_length_preserved possible_constants ts ts' ts'_mem]
+            exact arity_ok.left
+          . apply g.arguments_for_pre_term_list_arity_ok possible_constants ts _ ts' ts'_mem
+            exact arity_ok.right
+
+      theorem arguments_for_pre_term_list_arity_ok (g : StrictConstantMapping sig) (possible_constants : List sig.C) (ts : FiniteTreeList (SkolemFS sig) sig.C) (arity_ok : PreGroundTerm.arity_ok_list ts) : ∀ ts', ts' ∈ (g.arguments_for_pre_term_list possible_constants ts) -> PreGroundTerm.arity_ok_list (FiniteTreeList.fromList ts') := by
+        intro ts' ts'_mem
+        cases ts with
+        | nil => simp [arguments_for_pre_term_list] at ts'_mem; rw [ts'_mem]; simp [PreGroundTerm.arity_ok_list]
+        | cons hd tl =>
+          unfold PreGroundTerm.arity_ok_list at arity_ok
+          rw [Bool.and_eq_true] at arity_ok
+          unfold arguments_for_pre_term_list at ts'_mem
+          simp only [List.mem_flatMap, List.mem_map] at ts'_mem
+          rcases ts'_mem with ⟨arg_hd, arg_hd_mem, arg_tl, arg_tl_mem, ts'_eq⟩
+          rw [← ts'_eq]
+          unfold FiniteTreeList.fromList
+          unfold PreGroundTerm.arity_ok_list
+          rw [Bool.and_eq_true]
+          constructor
+          . apply g.arguments_for_pre_term_arity_ok possible_constants hd _ _ arg_hd_mem
+            exact arity_ok.left
+          . apply g.arguments_for_pre_term_list_arity_ok possible_constants tl _ _ arg_tl_mem
+            exact arity_ok.right
+
+    end
+
+    /- def arguments_for_term (g : StrictConstantMapping sig) (possible_constants : List sig.C) (t : GroundTerm sig) : List (GroundTerm sig) := -/
+    /-   (g.arguments_for_pre_term possible_constants t.val).attach.map (fun ⟨t', mem⟩ => -/
+    /-     ⟨t', g.arguments_for_pre_term_arity_ok possible_constants t.val t.property t' mem⟩ -/
+    /-   ) -/
+
+    def arguments_for_term_list (g : StrictConstantMapping sig) (possible_constants : List sig.C) (ts : List (GroundTerm sig)) : List (List (GroundTerm sig)) :=
+      (g.arguments_for_pre_term_list possible_constants (FiniteTreeList.fromList ts.unattach)).attach.map (fun ⟨ts', mem⟩ =>
+        have arity_ok := g.arguments_for_pre_term_list_arity_ok possible_constants (FiniteTreeList.fromList ts.unattach) (by
+          rw [← PreGroundTerm.arity_ok_list_iff_arity_ok_each_mem]
+          intro t t_mem
+          rw [FiniteTreeList.fromListToListIsId] at t_mem
+          unfold List.unattach at t_mem
+          rw [List.mem_map] at t_mem
+          rcases t_mem with ⟨t', _, t_eq⟩
+          rw [← t_eq]
+          exact t'.property
+        ) ts' mem
+
+        ts'.attach.map (fun ⟨t, mem⟩ =>
+          ⟨t, by
+            rw [← PreGroundTerm.arity_ok_list_iff_arity_ok_each_mem] at arity_ok
+            apply arity_ok
+            rw [FiniteTreeList.fromListToListIsId]
+            exact mem
+          ⟩
+        )
+      )
+
+    theorem apply_to_arguments_yields_original_term_list (g : StrictConstantMapping sig) (possible_constants : List sig.C) (ts : List (GroundTerm sig)) :
+        ∀ args, args ∈ g.arguments_for_term_list possible_constants ts ↔ ((∀ c, c ∈ (FiniteTree.leavesList (FiniteTreeList.fromList args.unattach)) -> c ∈ possible_constants) ∧ (args.map (fun arg => g.toConstantMapping.apply_ground_term arg) = ts)) := by
+      intro args
+
+      have := g.apply_to_arguments_yields_original_pre_term_list possible_constants (FiniteTreeList.fromList ts.unattach)
+
+      unfold arguments_for_term_list
+      constructor
+      . intro h
+        simp at h
+        rcases h with ⟨args', h, eq⟩
+        rw [← List.pmap_eq_map_attach] at eq
+        rw [← eq]
+
+        rw [this] at h
+        rw [FiniteTree.mapLeavesList_fromList_eq_fromList_map] at h
+        rw [← FiniteTreeList.eqIffFromListEq] at h
+        constructor
+        . intro c c_mem
+          unfold List.unattach at c_mem
+          rw [List.map_pmap] at c_mem
+          simp at c_mem
+          apply h.left
+          exact c_mem
+        . rw [← List.eq_iff_unattach_eq]
+          simp only [← h.right]
+          unfold ConstantMapping.apply_ground_term
+          unfold ConstantMapping.apply_pre_ground_term
+          rw [List.map_pmap]
+          unfold List.unattach
+          rw [List.map_pmap]
+          rw [List.pmap_eq_map]
+      . intro h
+        simp
+        exists args.unattach
+        exists (by
+          rw [this]
+          constructor
+          . exact h.left
+          . rw [← h.right]
+            rw [FiniteTree.mapLeavesList_fromList_eq_fromList_map]
+            rw [← FiniteTreeList.eqIffFromListEq]
+            unfold ConstantMapping.apply_ground_term
+            unfold ConstantMapping.apply_pre_ground_term
+            unfold List.unattach
+            simp
+        )
+        rw [← List.pmap_eq_map_attach]
+        rw [← List.eq_iff_unattach_eq]
+        unfold List.unattach
+        rw [List.map_pmap]
+        rw [List.pmap_eq_map]
+        simp
 
     variable [DecidableEq sig.P]
 
     def arguments_for_fact (g : StrictConstantMapping sig) (possible_constants : List sig.C) (f : Fact sig) : List (Fact sig) :=
-      (g.arguments_for_term_list possible_constants (FiniteTreeList.fromList f.terms)).attach.map (fun ⟨ts, mem⟩ =>
+      (g.arguments_for_term_list possible_constants f.terms).attach.map (fun ⟨ts, mem⟩ =>
         {
           predicate := f.predicate
           terms := ts
           arity_ok := by
-            rw [g.arguments_for_term_list_length_preserved _ _ ts mem]
-            rw [FiniteTreeList.fromListToListIsId]
-            exact f.arity_ok
+            unfold arguments_for_term_list at mem
+            rw [List.mem_map] at mem
+            rcases mem with ⟨ts', ts'_mem, ts_eq⟩
+            rw [← ts_eq]
+            simp only [List.length_map, List.length_attach]
+            rw [g.arguments_for_pre_term_list_length_preserved possible_constants (FiniteTreeList.fromList f.terms.unattach) ts'.val _]
+            . rw [FiniteTreeList.fromListToListIsId, List.length_unattach]
+              exact f.arity_ok
+            . unfold List.attach at ts'_mem
+              unfold List.attachWith at ts'_mem
+              rw [List.mem_pmap] at ts'_mem
+              rcases ts'_mem with ⟨_, ts'_mem, eq⟩
+              rw [← eq]
+              exact ts'_mem
         }
       )
 
@@ -445,7 +588,7 @@ section ArgumentsForImages
       unfold arguments_for_fact
       simp only [List.mem_map, List.mem_attach, true_and, Subtype.exists]
 
-      have := g.apply_to_arguments_yields_original_term_list possible_constants (FiniteTreeList.fromList f.terms)
+      have := g.apply_to_arguments_yields_original_term_list possible_constants f.terms
 
       constructor
       . intro h
@@ -457,13 +600,7 @@ section ArgumentsForImages
 
         specialize this ts
         rw [this] at mem
-        constructor
-        . exact mem.left
-        . have r := mem.right
-          rw [FiniteTree.mapLeavesList_fromList_eq_fromList_map] at r
-          rw [← FiniteTreeList.eqIffFromListEq] at r
-          unfold ConstantMapping.apply_ground_term
-          exact r
+        exact mem
       . intro h
         specialize this arg.terms
         exists arg.terms
@@ -474,12 +611,7 @@ section ArgumentsForImages
           . have r := h.right
             unfold ConstantMapping.apply_fact at r
             rw [Fact.ext_iff] at r
-            have r := r.right
-            simp only at r
-            rw [FiniteTree.mapLeavesList_fromList_eq_fromList_map]
-            rw [← FiniteTreeList.eqIffFromListEq]
-            unfold ConstantMapping.apply_ground_term at r
-            exact r
+            exact r.right
         )
         have r := h.right
         unfold ConstantMapping.apply_fact at r
@@ -896,7 +1028,7 @@ namespace RuleSet
         specialize isFunctionFree _ s_mem
         rcases isFunctionFree with ⟨c, s_eq⟩
         rw [← t_eq, s_eq]
-        simp [ConstantMapping.apply_ground_term, FiniteTree.mapLeaves, StrictConstantMapping.toConstantMapping]
+        simp [ConstantMapping.apply_ground_term, ConstantMapping.apply_pre_ground_term, FiniteTree.mapLeaves, StrictConstantMapping.toConstantMapping, GroundTerm.const]
       have f_func_free : ((UniformConstantMapping sig special_const).toConstantMapping.apply_fact f).isFunctionFree := by
         intro t t_mem
         exists special_const
@@ -909,11 +1041,11 @@ namespace RuleSet
         constructor
         . exact f_predicate
         . simp
-          intro c t t_mem c_eq
-          specialize every_t_special_const t t_mem
+          intro c t t_arity_ok t_mem c_eq
+          specialize every_t_special_const ⟨t, t_arity_ok⟩ t_mem
           rw [← c_eq]
           simp only [every_t_special_const]
-          simp [GroundTerm.toConst]
+          simp [GroundTerm.const, GroundTerm.toConst]
       . rw [Fact.toFact_after_toFunctionFreeFact_is_id]
     | succ n ih =>
       cases eq_node : cb.branch.infinite_list (n+1) with
@@ -1090,7 +1222,7 @@ namespace RuleSet
                         | var v =>
                           simp [GroundSubstitution.apply_var_or_const, StrictConstantMapping.apply_var_or_const]
                         | const c =>
-                          simp [GroundSubstitution.apply_var_or_const, StrictConstantMapping.apply_var_or_const, ConstantMapping.apply_ground_term, FiniteTree.mapLeaves, StrictConstantMapping.toConstantMapping]
+                          simp [GroundSubstitution.apply_var_or_const, StrictConstantMapping.apply_var_or_const, ConstantMapping.apply_ground_term, ConstantMapping.apply_pre_ground_term, FiniteTree.mapLeaves, StrictConstantMapping.toConstantMapping, GroundTerm.const]
                   . intro f f_mem
                     rcases f_mem with ⟨f_pred, f', f'_mem, f_eq⟩
                     rw [f_eq]
@@ -1143,7 +1275,7 @@ namespace RuleSet
                         simp only
                         split <;> simp
                     | const c =>
-                      simp only [StrictConstantMapping.apply_var_or_const, VarOrConst.skolemize, GroundSubstitution.apply_skolem_term, ConstantMapping.apply_ground_term, FiniteTree.mapLeaves, StrictConstantMapping.toConstantMapping]
+                      simp only [StrictConstantMapping.apply_var_or_const, VarOrConst.skolemize, GroundSubstitution.apply_skolem_term, ConstantMapping.apply_ground_term, ConstantMapping.apply_pre_ground_term, FiniteTree.mapLeaves, StrictConstantMapping.toConstantMapping, GroundTerm.const]
               . unfold PreTrigger.result at f_mem
                 simp only [List.get_eq_getElem, disj_index_zero] at f_mem
                 rw [List.getElem_map, ← List.inIffInToSet] at f_mem
@@ -1176,7 +1308,7 @@ namespace RuleSet
                       simp only
                       split <;> simp
                   | const c =>
-                    simp only [StrictConstantMapping.apply_var_or_const, VarOrConst.skolemize, GroundSubstitution.apply_skolem_term, ConstantMapping.apply_ground_term, FiniteTree.mapLeaves, StrictConstantMapping.toConstantMapping]
+                    simp only [StrictConstantMapping.apply_var_or_const, VarOrConst.skolemize, GroundSubstitution.apply_skolem_term, ConstantMapping.apply_ground_term, ConstantMapping.apply_pre_ground_term, FiniteTree.mapLeaves, StrictConstantMapping.toConstantMapping, GroundTerm.const]
 
   theorem filtered_cb_result_subset_mfaSet (rs : RuleSet sig) (finite : rs.rules.finite) (det : rs.isDeterministic) (special_const : sig.C) : ∀ {db : Database sig} (cb : ChaseBranch obs { rules := rs, db := db }), ((UniformConstantMapping sig special_const).toConstantMapping.apply_fact_set (fun f => f.predicate ∈ rs.predicates ∧ f ∈ cb.result)) ⊆ (rs.mfaSet finite det special_const) := by
     intro db cb f f_mem
@@ -1351,7 +1483,7 @@ namespace RuleSet
     . exact res_filtered_finite
 
   def isMfa [Inhabited sig.C] (rs : RuleSet sig) (finite : rs.rules.finite) (det : rs.isDeterministic) : Prop :=
-    ∀ t, t ∈ (rs.mfaSet finite det default).terms -> ¬ t.cyclic
+    ∀ t, t ∈ (rs.mfaSet finite det default).terms -> ¬ t.val.cyclic
 
   theorem terminates_of_isMfa [Inhabited sig.C] (rs : RuleSet sig) (rs_finite : rs.rules.finite) (det : rs.isDeterministic) : rs.isMfa rs_finite det -> rs.terminates obs := by
     intro isMfa
